proofs/hol_light/x86_64/proofs/mlkem_poly_basemul_acc_montgomery_cached_k4.ml
@@ -1633,6 +1633,22 @@ let mlkem_basemul_k4_mc =
 let mlkem_basemul_k4_tmc = define_trimmed "mlkem_basemul_k4_tmc" mlkem_basemul_k4_mc;;
 let mlkem_basemul_k4_tmc_EXEC = X86_MK_CORE_EXEC_RULE mlkem_basemul_k4_tmc;;
 
+let LENGTH_MLKEM_BASEMUL_K4_TMC =
+  REWRITE_CONV[mlkem_basemul_k4_tmc] `LENGTH mlkem_basemul_k4_tmc`
+  |> CONV_RULE(RAND_CONV LENGTH_CONV);;
+
+let MLKEM_BASEMUL_K4_POSTAMBLE_LENGTH = new_definition
+  `MLKEM_BASEMUL_K4_POSTAMBLE_LENGTH = 1`;;
+
+let MLKEM_BASEMUL_K4_CORE_END = new_definition
+  `MLKEM_BASEMUL_K4_CORE_END = LENGTH mlkem_basemul_k4_tmc - MLKEM_BASEMUL_K4_POSTAMBLE_LENGTH`;;
+
+let LENGTH_SIMPLIFY_CONV =
+  REWRITE_CONV[LENGTH_MLKEM_BASEMUL_K4_TMC;
+              MLKEM_BASEMUL_K4_CORE_END;
+              MLKEM_BASEMUL_K4_POSTAMBLE_LENGTH] THENC
+  NUM_REDUCE_CONV THENC REWRITE_CONV [ADD_0];;
+
 (* Enable simplification of word_subwords by default.
    Nedded to prevent the symbolic simulation to explode
    as we add more instructions. *)
@@ -1706,7 +1722,7 @@ let MLKEM_BASEMUL_K4_CORRECT = prove(
         aligned 32 src2t /\
         aligned 32 dst /\
         ALL (nonoverlapping (dst, 512)) [(src1, 2048); (src2, 2048); (src2t, 1024)] /\
-        nonoverlapping (dst, 512) (word pc, 5202)
+        nonoverlapping (dst, 512) (word pc, LENGTH mlkem_basemul_k4_tmc)
         ==> ensures x86
               (\s. bytes_loaded s (word pc) (BUTLAST mlkem_basemul_k4_tmc) /\
                    read RIP s = word pc /\
@@ -1774,7 +1790,7 @@ let MLKEM_BASEMUL_K4_CORRECT = prove(
                    (!i. i < 16 ==> !j. j < 8
                         ==> read(memory :> bytes16
                              (word_add src2t (word (768 + 32*j + 2*i)))) s = dz3 i j))
-              (\s. read RIP s = word (pc + 5202) /\
+              (\s. read RIP s = word (pc + MLKEM_BASEMUL_K4_CORE_END) /\
                    (!i. i < 16 ==> !j. j < 4
                         ==> (let j' = 2*j in
                               (abs(ival(a0 i j')) <= &2 pow 12  /\
@@ -1835,6 +1851,7 @@ let MLKEM_BASEMUL_K4_CORRECT = prove(
                           ZMM8; ZMM9; ZMM10; ZMM11; ZMM12; ZMM13; ZMM14] ,,
                MAYCHANGE [memory :> bytes(dst, 512)])`,
 
+  CONV_TAC LENGTH_SIMPLIFY_CONV THEN
   REWRITE_TAC [MAYCHANGE_REGS_AND_FLAGS_PERMITTED_BY_ABI;
     NONOVERLAPPING_CLAUSES; ALL; C_ARGUMENTS; fst mlkem_basemul_k4_tmc_EXEC] THEN
   REPEAT STRIP_TAC THEN
@@ -2026,7 +2043,9 @@ let MLKEM_BASEMUL_K4_NOIBT_SUBROUTINE_CORRECT = prove(
                             ) (mod &3329)))
               (MAYCHANGE [RSP] ,, MAYCHANGE_REGS_AND_FLAGS_PERMITTED_BY_ABI ,,
                MAYCHANGE [memory :> bytes(dst, 512)])`,
-  X86_PROMOTE_RETURN_NOSTACK_TAC mlkem_basemul_k4_tmc MLKEM_BASEMUL_K4_CORRECT);;
+  CONV_TAC LENGTH_SIMPLIFY_CONV THEN
+  X86_PROMOTE_RETURN_NOSTACK_TAC mlkem_basemul_k4_tmc
+    (CONV_RULE LENGTH_SIMPLIFY_CONV MLKEM_BASEMUL_K4_CORRECT));;
 
 (* NOTE: This must be kept in sync with the CBMC specification
  * in mlkem/src/native/x86_64/src/arith_native_x86_64.h *)
@@ -2168,4 +2187,117 @@ let MLKEM_BASEMUL_K4_SUBROUTINE_CORRECT = prove(
               (MAYCHANGE [RSP] ,, MAYCHANGE_REGS_AND_FLAGS_PERMITTED_BY_ABI ,,
                MAYCHANGE [memory :> bytes(dst, 512)])`,
   MATCH_ACCEPT_TAC(ADD_IBT_RULE MLKEM_BASEMUL_K4_NOIBT_SUBROUTINE_CORRECT));;
+
+(* ------------------------------------------------------------------------- *)
+(* Constant-time and memory safety proof.                                    *)
+(* ------------------------------------------------------------------------- *)
+
+needs "x86/proofs/consttime.ml";;
+needs "x86_64/proofs/subroutine_signatures.ml";;
+needs "common/consttime_utils.ml";;
+
+let full_spec,public_vars = mk_safety_spec
+    ~keep_maychanges:true
+    (assoc "mlkem_basemul_k4" subroutine_signatures)
+    MLKEM_BASEMUL_K4_CORRECT
+    mlkem_basemul_k4_tmc_EXEC;;
+
+let MLKEM_BASEMUL_K4_SAFE = time prove
+ (`exists f_events.
+       forall e src1 src2 src2t dst pc.
+           aligned 32 src1 /\
+           aligned 32 src2 /\
+           aligned 32 src2t /\
+           aligned 32 dst /\
+           ALL (nonoverlapping (dst,512)) [src1,2048; src2,2048; src2t,1024] /\
+           nonoverlapping (dst,512) (word pc,LENGTH mlkem_basemul_k4_tmc)
+           ==> ensures x86
+               (\s.
+                    bytes_loaded s (word pc)
+                      (BUTLAST mlkem_basemul_k4_tmc) /\
+                    read RIP s = word pc /\
+                    C_ARGUMENTS [dst; src1; src2; src2t] s /\
+                    read events s = e)
+               (\s.
+                    read RIP s = word (pc + MLKEM_BASEMUL_K4_CORE_END) /\
+                    (exists e2.
+                         read events s = APPEND e2 e /\
+                         e2 = f_events src1 src2 src2t dst pc /\
+                         memaccess_inbounds e2
+                           [src1,2048; src2,2048; src2t,1024; dst,512]
+                           [dst,512]))
+               (MAYCHANGE [events] ,,
+              MAYCHANGE [RIP] ,,
+              MAYCHANGE [RAX] ,,
+              MAYCHANGE
+              [ZMM0; ZMM1; ZMM2; ZMM3; ZMM4; ZMM5; ZMM6; ZMM7;
+               ZMM8; ZMM9; ZMM10; ZMM11; ZMM12; ZMM13; ZMM14] ,,
+              MAYCHANGE [memory :> bytes (dst,512)])`,
+  ASSERT_CONCL_TAC full_spec THEN
+  CONV_TAC LENGTH_SIMPLIFY_CONV THEN
+  PROVE_SAFETY_SPEC_TAC ~public_vars:public_vars mlkem_basemul_k4_tmc_EXEC);;
+
+let MLKEM_BASEMUL_K4_NOIBT_SUBROUTINE_SAFE = time prove
+ (`exists f_events.
+       forall e src1 src2 src2t dst pc stackpointer returnaddress.
+          aligned 32 src1 /\
+          aligned 32 src2 /\
+          aligned 32 src2t /\
+          aligned 32 dst /\
+          ALL (nonoverlapping (dst,512)) [src1,2048; src2,2048; src2t,1024] /\
+          nonoverlapping (dst,512) (word pc,LENGTH mlkem_basemul_k4_tmc) /\
+          nonoverlapping (stackpointer, 8) (dst, 512)
+          ==> ensures x86
+               (\s.
+                    bytes_loaded s (word pc) mlkem_basemul_k4_tmc /\
+                    read RIP s = word pc /\
+                    read RSP s = stackpointer /\
+                    read (memory :> bytes64 stackpointer) s = returnaddress /\
+                    C_ARGUMENTS [dst; src1; src2; src2t] s /\
+                    read events s = e)
+               (\s. read RIP s = returnaddress /\
+                    read RSP s = word_add stackpointer (word 8) /\
+                    (exists e2.
+                         read events s = APPEND e2 e /\
+                         e2 = f_events src1 src2 src2t dst pc
+                                       stackpointer returnaddress /\
+                         memaccess_inbounds e2
+                           [src1,2048; src2,2048; src2t,1024;
+                            dst,512; stackpointer,8]
+                           [dst,512; stackpointer,8]))
+               (\s s'. true)`,
+  X86_PROMOTE_RETURN_NOSTACK_TAC mlkem_basemul_k4_tmc
+    (CONV_RULE LENGTH_SIMPLIFY_CONV MLKEM_BASEMUL_K4_SAFE) THEN
+  DISCHARGE_SAFETY_PROPERTY_TAC);;
+
+let MLKEM_BASEMUL_K4_SUBROUTINE_SAFE = time prove
+ (`exists f_events.
+       forall e src1 src2 src2t dst pc stackpointer returnaddress.
+          aligned 32 src1 /\
+          aligned 32 src2 /\
+          aligned 32 src2t /\
+          aligned 32 dst /\
+          ALL (nonoverlapping (dst,512)) [src1,2048; src2,2048; src2t,1024] /\
+          nonoverlapping (dst,512) (word pc,LENGTH mlkem_basemul_k4_mc) /\
+          nonoverlapping (stackpointer, 8) (dst, 512)
+          ==> ensures x86
+               (\s.
+                    bytes_loaded s (word pc) mlkem_basemul_k4_mc /\
+                    read RIP s = word pc /\
+                    read RSP s = stackpointer /\
+                    read (memory :> bytes64 stackpointer) s = returnaddress /\
+                    C_ARGUMENTS [dst; src1; src2; src2t] s /\
+                    read events s = e)
+               (\s. read RIP s = returnaddress /\
+                    read RSP s = word_add stackpointer (word 8) /\
+                    (exists e2.
+                         read events s = APPEND e2 e /\
+                         e2 = f_events src1 src2 src2t dst pc
+                                       stackpointer returnaddress /\
+                         memaccess_inbounds e2
+                           [src1,2048; src2,2048; src2t,1024;
+                            dst,512; stackpointer,8]
+                           [dst,512; stackpointer,8]))
+               (\s s'. true)`,
+  MATCH_ACCEPT_TAC(ADD_IBT_RULE MLKEM_BASEMUL_K4_NOIBT_SUBROUTINE_SAFE));;
 
